add well-formedness

src/BPlusTree.v
@@ -2,11 +2,18 @@ From iris.algebra Require Import numbers.
 From iris.heap_lang Require Export proofmode notation.
 From iris.proofmode Require Export proofmode.
 From iris.prelude Require Import options.
+Import Decidable.
 
 Section nary_tree.
   Context (A:Set).
-  Context (beq_A : A -> A -> bool).
+  Context (eqb_A : A -> A -> bool).
+  Hypothesis (eqb_refl : forall a, eqb_A a a = true).
+  Hypothesis (eqb_eq : forall a a', eqb_A a a' = true <-> a = a').
+  Hypothesis (eqb_dec : forall a a', decidable (eqb_A a a' = true)).
   Context (ord_A : A -> A -> Prop).
+  Definition ordeq_A (a a' : A) :=
+    eqb_A a a' = true \/ ord_A a a'.
+  Hypothesis (ord_trans : Transitive ord_A).
 
   Inductive nary_tree : Set :=
   | leaf (interval : A * A) (l : list A) : nary_tree
@@ -28,41 +35,74 @@ Section nary_tree.
              end) trees)
     end.
 
+  Fixpoint list_sorted (l : list A) :=
+    match l with
+    | [] => True
+    | x :: l =>
+        match l with
+        | [] => True
+        | y :: _ => ord_A x y /\ list_sorted l
+        end
+    end.
+
   Fixpoint nary_tree_wf (t : nary_tree) :=
     match t with
-    | leaf (low, high) vals => Forall (fun a' => ord_A low a' /\ ord_A a' high) vals
+    | leaf (low, high) vals =>
+        ordeq_A low high /\
+          hd low vals = low /\
+          List.last vals high = high /\
+          list_sorted vals
     | node (low, high) trees =>
-        (fix nary_tree_wf_aux (l : list nary_tree) : Prop :=
-           match l with
-           | [] => True
-           | t :: ts =>
-               nary_tree_wf t /\
+        let intervals :=
+          map (fun t =>
                  match t with
-                 | leaf (low', high') _ => ord_A low low' /\ ord_A high' high
-                 | node (low', high') _ => ord_A low low' /\ ord_A high' high
-                 end /\
-                 nary_tree_wf_aux ts
-           end) trees
+                 | leaf (low', high') _
+                 | node (low', high') _ => (low', high')
+                 end)
+            trees
+        in
+        Forall (fun (interval : A * A) =>
+                  let (low', high') := interval in
+                  ord_A low low' /\ ord_A high' high)
+          intervals /\
+          (fix trees_wf (l : list nary_tree) : Prop :=
+             match l with
+             | [] => True
+             | t :: rest => nary_tree_wf t /\ trees_wf rest
+             end) trees /\
+          (fix intervals_sorted (l : list (A * A)) : Prop :=
+             match l with
+             | [] => True
+             | (_, high') :: rest =>
+                 match rest with
+                 | [] => True
+                 | (low', high'') :: rest' =>
+                     ord_A high' low'
+                 end /\ intervals_sorted rest
+             end) intervals
     end.
 
   Lemma nary_tree_wf_branches interval branches (wf : nary_tree_wf (node interval branches)) :
     Forall (fun t => nary_tree_wf t) branches.
   Proof.
+    cbn in wf.
+    destruct interval as [low high].
+    destruct wf as (_ & wf_branches & _).
     induction branches.
     - done.
-    - cbn in wf.
-      destruct interval as [low high].
-      destruct wf as (wf_a & ? & wf_branches).
+    - destruct wf_branches as (wf_a & wf_branches).
       constructor; [done|].
       apply IHbranches.
       done.
   Qed.
 
-  Record Tree : Set :=
-    mkTree {
-        tree : nary_tree;
-        tree_wf : nary_tree_wf tree
-      }.
+  Axiom destruct_list_back : forall (l : list A), {x:A & {init:list A | l = init ++ [x] }}+{l = [] }.
+
+  Definition nary_tree_interval t : (A * A) :=
+    match t with
+    | leaf i _ => i
+    | node i _ => i
+    end.
 
   Fixpoint size (t : nary_tree) : nat :=
     match t with
@@ -73,18 +113,96 @@ Section nary_tree.
   Fixpoint In_list (v : A) (l : list A) :=
     match l with
     | [] => false
-    | x :: xs => orb (beq_A x v) (In_list v xs)
+    | x :: xs => orb (eqb_A x v) (In_list v xs)
     end.
+
+  Lemma In_list_split : ∀ (x : A) (l : list A), In_list x l = true → ∃ l1 l2 : list A, l = l1 ++ x :: l2.
+  Admitted.
+
+  Lemma In_list_sorted_interval l target : list_sorted l -> In_list target l = true -> ordeq_A (hd target l) target.
+  Proof using ord_trans eqb_refl eqb_eq eqb_dec.
+    intros sorted_l in_target_l.
+    destruct l; [done|].
+    cbn.
+    apply (orb_prop) in in_target_l.
+    destruct in_target_l.
+    - left.
+      done.
+    - apply In_list_split in H.
+      destruct H as (l' & ? & ->).
+      induction l'.
+      + destruct sorted_l as (? & _).
+        right.
+        done.
+      + apply IHl'.
+        destruct sorted_l as (ord_a_a0 & sorted_l).
+        cbn in sorted_l.
+        cbn.
+        destruct (l' ++ target :: x); [done|].
+        destruct sorted_l as (ord_a0_a1 & ?).
+        split; [|done].
+        apply (ord_trans _ _ _ ord_a_a0 ord_a0_a1).
+  Qed.
 
   Fixpoint In_tree (v : A) (t : nary_tree) {struct t} : bool :=
     match t with
     | leaf _ l => In_list v l
-    | node _ l => (fix In_aux (l : list nary_tree) :=
-                  match l with
-                  | [] => false
-                  | t :: ts => orb (In_tree v t) (In_aux ts)
-                  end) l
+    | node _ l =>
+        (fix In_aux (l : list nary_tree) :=
+           match l with
+           | [] => false
+           | t :: ts => orb (In_tree v t) (In_aux ts)
+           end) l
     end.
+
+  Lemma nary_tree_in_interval_not_in_others target interval branch branches (wf : nary_tree_wf (node interval (branch :: branches))) :
+    ordeq_A (fst (nary_tree_interval branch)) target /\ ordeq_A target (snd (nary_tree_interval branch)) ->
+    false = (fix In_aux (l : list nary_tree) :=
+           match l with
+           | [] => false
+           | t :: ts => orb (In_tree target t) (In_aux ts)
+           end) branches.
+  Proof.
+    intros (? & ?).
+    destruct interval.
+    cbn in wf.
+    destruct wf as (_ & [wf_branch wf_branches] & wf).
+    induction branches as [|branch' branches]; [done|].
+    destruct branch, branch'.
+    - destruct interval as (low & high), interval0 as (low' & high').
+      destruct wf_branches as [wf_branch' wf_branches].
+      specialize (IHbranches wf_branches).
+      cbn in wf.
+      destruct wf as (ord_high_low' & wf).
+      destruct wf_branch' as (ordeq_low'_high' & _ & _ & sorted_l0).
+      assert (ord_A high high') as ord_high_high'.
+      { destruct ordeq_low'_high' as [eqb_low'_high' | ord_low'_high'].
+        - apply eqb_eq in eqb_low'_high'; subst.
+          done.
+        - apply (ord_trans _ _ _ ord_high_low' ord_low'_high'). }
+      assert (match
+                 map
+                   (λ t : nary_tree,
+                      match t with
+                      | leaf (low', high') _ | node (low', high') _ => (low', high')
+                      end) branches
+               with
+               | [] => True
+               | (low', _) :: _ => ord_A high low'
+               end).
+      { destruct branches; [done|].
+        destruct wf as (wf & _).
+        destruct n, interval;
+          cbn in *;
+          apply (ord_trans _ _ _ ord_high_high' wf). }
+      specialize (IHbranches (conj H1 (proj2 wf)));
+        clear H1 wf.
+      rewrite <- IHbranches, orb_false_r.
+      destruct (In_list target l0) eqn:?; [|done];
+        exfalso.
+      specialize (In_list_sorted_interval _ _ sorted_l0 Heqb)as ord_low'_target.
+  Admitted.
+
 End nary_tree.
 
 Section bplus_tree.
@@ -107,9 +225,9 @@ Section bplus_tree.
   Variable (ninf pinf : tval).
   Definition teqb := Nat.eqb.
   Definition tord := Nat.lt.
-  Axiom pinf_max : forall v, (v < pinf).
-  Axiom ninf_minax : forall v, (ninf < v).
-  Definition tree_spec := Tree tval tord.
+  Axiom pinf_max : forall v, (tord v pinf).
+  Axiom ninf_minax : forall v, (tord ninf v).
+  Definition tree_spec := nary_tree tval.
 
   Section bplus_tree_model.
     Context `{!heapGS Σ}.
@@ -126,9 +244,9 @@ Section bplus_tree.
 
     Definition leaf_node v (t : tree_spec) (interval : tval * tval) (vals : list tval) :=
       let (low, high) := interval in
-      (∃ (ptr : loc) (lhd : val), ⌜ size _ (tree _ _ t) < b ⌝ ∗ ⌜ v = token_leaf_v #ptr ⌝ ∗ ptr ↦ ((#low, #high), lhd) ∗ is_list lhd (map (fun (x : tval) => #x) vals))%I.
+      (∃ (ptr : loc) (lhd : val), ⌜ size _ t < b ⌝ ∗ ⌜ v = token_leaf_v #ptr ⌝ ∗ ptr ↦ ((#low, #high), lhd) ∗ is_list lhd (map (fun (x : tval) => #x) vals))%I.
 
-    Definition branch_node v (t : nary_tree tval) (* (t_wf : nary_tree_wf _ tord t) *) (interval : tval * tval) ts node_size_min (is_node : forall (_ : val) (t : nary_tree tval), nary_tree_wf _ _ t -> iProp) :=
+    Definition branch_node v (t : nary_tree tval) (* (t_wf : nary_tree_wf _ tord t) *) (interval : tval * tval) ts node_size_min (is_node : forall (_ : val) (t : nary_tree tval), (* nary_tree_wf _ _ t ->  *)iProp) :=
       let (low, high) := interval in
       (∃ (ptr : loc) l (ns : list val),
           (* these two should be moved to spec *)
@@ -142,47 +260,44 @@ Section bplus_tree.
           ((fix branch_node_list (ns : list val) (ts : list tree_spec) {struct ts} : iProp :=
               match ns, ts with
               | [], [] => True
-              | n :: ns, t :: ts => is_node n (tree _ _ t) (tree_wf _ _ t) ∗ branch_node_list ns ts
+              | n :: ns, t :: ts => is_node n t ∗ branch_node_list ns ts
               | _, _ => False
               end)
              ns ts))%I.
 
-    Fixpoint is_node (v : val) (t : nary_tree tval) (t_wf : nary_tree_wf _ _ t) {struct t} : iProp :=
-      match t as t0 return t = t0 -> iProp with
-      | leaf _ interval l => fun _ => leaf_node v {| tree := t; tree_wf := t_wf |} interval l
-      | node _ interval ts => fun t_t0 =>
-          let t_wf' := nary_tree_wf_branches
-                         tval
-                         tord
-                         interval
-                         ts
-                         (eq_rect
-                            t
-                            _
-                            t_wf
-                            (node _ interval ts)
-                            t_t0) in
-          let trees := ((fix is_node_list (ts : list (nary_tree tval)) (ts_wf : Forall (fun t => nary_tree_wf _ _ t) ts) : list tree_spec :=
-              match ts as ts0 return ts = ts0 -> list tree_spec with
-              | [] => fun _ => []
-              | t' :: ts' =>
-                  fun ts_ts0 =>
-                    let ts_wf_cons := Forall_cons_1
-                                        (fun x => nary_tree_wf _ _ x)
-                                        t'
-                                        ts'
-                                        (eq_rect ts _ ts_wf (t' :: ts') ts_ts0) in
-                    let t'_wf := proj1 ts_wf_cons in
-                    let ts'_wf := proj2 ts_wf_cons in
-                    {| tree := t'; tree_wf := t'_wf |} :: is_node_list ts' ts'_wf
-              end eq_refl) ts t_wf') in
-          branch_node v t interval trees (b / 2) is_node
-      end eq_refl%I.
-
-    Definition is_bplus_tree (v : val) (t : tree_spec) (* (t_wf : nary_tree_wf _ tord t) *) : iProp :=
+    Fixpoint is_node (v : val) (t : nary_tree tval) (* (t_wf : nary_tree_wf _ _ t) *) {struct t} : iProp :=
       match t with
-      | leaf _ interval l => leaf_node v t interval l
-      | node _ interval ts => branch_node v t interval ts 2 is_node
+      | leaf _ interval l => leaf_node v t (* t_wf *) interval l
+      | node _ interval ts =>
+         let (low, high) := interval in
+         (∃ (ptr : loc) l (ns : list val),
+             (* these two should be moved to spec *)
+             ⌜ size _ t >= b ⌝ ∗
+             ⌜ b / 2 <= length ns <= b ⌝ ∗
+             (* the rest are fine ? *)
+             ⌜ v = token_branch_v #ptr ⌝ ∗
+             ⌜ length ns = length ts ⌝ ∗
+             ptr ↦ (((#low), (#high)), l) ∗
+             is_list l ns ∗
+             ((fix branch_node_list (ns : list val) (ts : list tree_spec) {struct ts} : iProp :=
+                 match ns, ts with
+                 | [], [] => True
+                 | n :: ns, t :: ts => is_node n t ∗ branch_node_list ns ts
+                 | _, _ => False
+                 end)
+                ns ts))
+           end%I.
+
+    Record Tree : Set :=
+      mkTree {
+          tree : nary_tree tval;
+          tree_wf : nary_tree_wf _ teqb tord tree
+        }.
+
+    Definition is_bplus_tree (v : val) (t : Tree) : iProp :=
+      match (tree t) with
+      | leaf _ interval l => leaf_node v (tree t) interval l
+      | node _ interval ts => branch_node v (tree t) interval ts 2 is_node
       end%I.
 
   End bplus_tree_model.
@@ -255,11 +370,15 @@ Section bplus_tree.
     Hypothesis bpos : 0 < b.
 
     Definition empty_tree := leaf tval (ninf, pinf) [].
-    Lemma empty_tree_wf : nary_tree_wf _ tord empty_tree.
-    Proof. apply Forall_nil_2. Qed.
+    Lemma empty_tree_wf : nary_tree_wf _ teqb tord empty_tree.
+    Proof.
+      repeat split; auto.
+      right.
+      apply (pinf_max ninf).
+    Qed.
 
     Theorem new_bplus_tree_spec:
-      {{{ True }}} new_bplus_tree #() {{{ v, RET v; is_bplus_tree b v empty_tree (* empty_tree_wf *) }}}.
+      {{{ True }}} new_bplus_tree #() {{{ v, RET v; is_bplus_tree b v {| tree := empty_tree; tree_wf := empty_tree_wf |} }}}.
     Proof using bpos.
       iIntros (Φ) "_ HPost".
       wp_lam; wp_alloc ptr; wp_pures.
@@ -271,8 +390,8 @@ Section bplus_tree.
       done.
     Qed.
 
-    Lemma tree_leaf_token_leaf v low high l (* (wf : (nary_tree_wf _ _ (leaf _ (low, high) l))) *):
-      is_bplus_tree b v (leaf _ (low, high) l) (* wf *) ⊢ ∃ x, ⌜ v = token_leaf_v x ⌝.
+    Lemma tree_leaf_token_leaf v low high l (wf : (nary_tree_wf _ _ _ (leaf _ (low, high) l))):
+      is_bplus_tree b v {| tree := leaf _ (low, high) l; tree_wf := wf |} ⊢ ∃ x, ⌜ v = token_leaf_v x ⌝.
     Proof.
       iIntros "Hv".
       iDestruct "Hv" as (? ?) "[% [% Hv]]".
@@ -280,8 +399,8 @@ Section bplus_tree.
       done.
     Qed.
 
-    Lemma tree_node_token_branch v low high l (* (wf : nary_tree_wf _ _ (node _ (low, high) l)) *):
-      is_bplus_tree b v (node _ (low, high) l) (* wf *) ⊢ ∃ x, ⌜ v = token_branch_v x ⌝.
+    Lemma tree_node_token_branch v low high l (wf : nary_tree_wf _ _ _ (node _ (low, high) l)):
+      is_bplus_tree b v {| tree := node _ (low, high) l; tree_wf := wf |} ⊢ ∃ x, ⌜ v = token_branch_v x ⌝.
     Proof.
       iIntros "Hv".
       iDestruct "Hv" as (? ? ? ?) "(_ & ? & _)".
@@ -353,13 +472,14 @@ Section bplus_tree.
             done.
     Qed.
 
-    Theorem search_bplus_tree_spec (t : tree_spec) (* (wf : nary_tree_wf _ _ t) *) (v : val) (target : nat) :
-      {{{ is_bplus_tree b v t (* wf *) }}} search_bplus_tree (v, #target)%V {{{ r, RET r; ⌜ r = #(In_tree _ teqb target t) ⌝ ∗ is_bplus_tree b v t (* wf *) }}}.
+    Theorem search_bplus_tree_spec (t : Tree) (v : val) (target : nat) :
+      {{{ is_bplus_tree b v t }}} search_bplus_tree (v, #target)%V {{{ r, RET r; ⌜ r = #(In_tree _ teqb target (tree t)) ⌝ ∗ is_bplus_tree b v t }}}.
     Proof using bpos.
       iIntros (Φ) "Hv HPost".
       iLöb as "IH" forall (v t).
-      
-      destruct t as [(low & high)|(low & high) ts].
+
+      destruct t.
+      destruct (tree0) as [(low & high)|(low & high) ts] eqn:?.
       - iPoseProof (tree_leaf_token_leaf with "Hv") as (?) "->".
         iDestruct "Hv" as (? ?) "(% & % & Hptr & Hlhd)".
         assert (x = #ptr) by (unfold token_leaf_v in H0; congruence); subst.
@@ -387,7 +507,7 @@ Section bplus_tree.
           destruct (bool_decide (Z.le (Z.of_nat low') (Z.of_nat target))) eqn:?; wp_pures.
           * destruct (bool_decide (Z.le (Z.of_nat target) (Z.of_nat high'))) eqn:?; wp_pures.
             -- iClear "IH'".
-               iApply ("IH" $! (token_leaf_v #ptr') (leaf _ (low', high') l) with "[Hptr' Hleaves]").
+               iApply ("IH" $! (token_leaf_v #ptr') {| tree := (leaf _ (low', high') l); tree_wf := _ |} with "[Hptr' Hleaves]").
                { iExists ptr', leaves.
                  iSplitR; [done|].
                   iSplitR; [done|].
@@ -398,10 +518,42 @@ Section bplus_tree.
                 iApply "HPost".
                 iSplitR.
                 { iPureIntro.
-                  cbn in *.
-                  
-                
-    Qed.
+                  cbn.
+                  apply bool_decide_eq_true_1 in Heqb0.
+                  apply bool_decide_eq_true_1 in Heqb1.
+                  assert (low' <= target) by lia.
+                  assert (target <= high') by lia.
+                  assert (ordeq_A _ teqb tord low' target).
+                  { destruct H5.
+                    - left.
+                      apply Nat.eqb_refl.
+                    - right.
+                      unfold tord.
+                      lia. }
+                  assert (ordeq_A _ teqb tord target high').
+                  { destruct H6.
+                    - left.
+                      apply Nat.eqb_refl.
+                    - right.
+                      unfold tord.
+                      lia. }
+                  rewrite <- (nary_tree_in_interval_not_in_others _ _ _ target (low, high) (leaf tval (low', high') l) trest tree_wf0 (conj H7 H8)).
+                  rewrite orb_false_r.
+                  done. }
+                iExists ptr, (InjRV #l0), (token_leaf_v #ptr' :: nrest).
+                iSplitR; [done|].
+                iSplitR; [done|].
+                iSplitR; [done|].
+                iSplitR; [done|].
+                iSplitL "Hptr"; [done|].
+                iSplitL "Hl0 Hnrest".
+                { iExists l0, hd'.
+                  iFrame.
+                  done. }
+                iSplitL "Htree"; [done|].
+                done.
+            --
+    Admitted.
 
   End bplus_tree_proofs.
 End bplus_tree.
